Compiler/CompilationModel/ScopeValidation.lean
@@ -359,7 +359,7 @@ def validateScopedExprIdentifiers
       ensureDynamicParam rhsName
   | Expr.add a b | Expr.sub a b | Expr.mul a b | Expr.div a b | Expr.sdiv a b | Expr.mod a b | Expr.smod a b |
     Expr.bitAnd a b | Expr.bitOr a b | Expr.bitXor a b | Expr.shl a b | Expr.shr a b |
-    Expr.sar a b | Expr.signextend a b |
+    Expr.sar a b | Expr.signextend a b | Expr.byte a b |
     Expr.eq a b | Expr.ge a b | Expr.gt a b | Expr.sgt a b | Expr.lt a b | Expr.slt a b | Expr.le a b |
     Expr.wMulDown a b => do
       validateScopedExprIdentifiers context params paramScope dynamicParams localScope constructorArgCount a
