Compiler/CompilationModel/ValidationCalls.lean
@@ -233,7 +233,7 @@ def validateInternalCallShapesInExpr
       validateInternalCallShapesInExpr functions callerName innerIndex
   | Expr.add a b | Expr.sub a b | Expr.mul a b | Expr.div a b | Expr.sdiv a b | Expr.mod a b | Expr.smod a b |
     Expr.bitAnd a b | Expr.bitOr a b | Expr.bitXor a b | Expr.shl a b | Expr.shr a b |
-    Expr.sar a b | Expr.signextend a b |
+    Expr.sar a b | Expr.signextend a b | Expr.byte a b |
     Expr.eq a b | Expr.ge a b | Expr.gt a b | Expr.sgt a b | Expr.lt a b | Expr.slt a b | Expr.le a b |
     Expr.logicalAnd a b | Expr.logicalOr a b |
     Expr.wMulDown a b | Expr.wDivUp a b | Expr.min a b | Expr.max a b |
@@ -506,7 +506,7 @@ def validateExternalCallTargetsInExpr
       validateExternalCallTargetsInExpr externals context innerIndex
   | Expr.add a b | Expr.sub a b | Expr.mul a b | Expr.div a b | Expr.sdiv a b | Expr.mod a b | Expr.smod a b |
     Expr.bitAnd a b | Expr.bitOr a b | Expr.bitXor a b | Expr.shl a b | Expr.shr a b |
-    Expr.sar a b | Expr.signextend a b |
+    Expr.sar a b | Expr.signextend a b | Expr.byte a b |
     Expr.eq a b | Expr.ge a b | Expr.gt a b | Expr.sgt a b | Expr.lt a b | Expr.slt a b | Expr.le a b |
     Expr.logicalAnd a b | Expr.logicalOr a b |
     Expr.wMulDown a b | Expr.wDivUp a b | Expr.min a b | Expr.max a b |
